

# 3

$$P(x<2) = F(2) = 1 - e^{-2\lambda}$$

令
$$1-e^{-2\hat\lambda} = \frac m n$$

$$\hat\lambda = - \frac 1 2 \ln{(1- \frac m n)}$$

# 6

## 矩估计


$$
\begin{cases}
\frac 1 n \sum_{i=1}^n x_i = e^{\hat\mu+\hat\sigma^2/2} \\
\frac 1 n \sum_{i=1}^n x_i^2 = e^{2\hat\mu+2\hat\sigma^2}
\end{cases}
$$
解得：
$$ \begin{cases}
\hat{\mu}=2\mathrm{ln}\overline{x}-\frac{1}{2}\mathrm{ln} A_{2}\\
\hat{\sigma}^{2}=\mathrm{ln} A_{2}-2\mathrm{ln} \overline{x}
\end{cases}$$
其中$A_{2} =\frac{1}{n}\sum_{i=1}^{n}x_{i}^{2}$

## 最大似然估计

$$
\begin{align}
\ln(L(\theta)) 
&= -n\hat\sigma -\sum_{i=1}^n x_i - \sum_{i=1}^n\left\{\frac{(\ln x_i-\mu)^{2}}{2\sigma^{2}}\right\}
\end{align}$$

分别求偏导，令其为0，得到：
$$\widehat\mu=\frac{1}{n}\sum_{i=1}^{n}\ln x_{i},\widehat\sigma^{2}=\frac{1}{n}\sum_{i=1}^{n}\left(\ln x_{i}-\widehat\mu\right)^{2}$$

# 11

$$
\begin{align}
\ln(L(\theta)) 
&= \sum_{i=1}^n (ln(\theta) \times I_{0 \leq x_i < 1}(x_i) + ln(1-\theta) \times (1 - I_{0 \leq x_i < 1}(x_i))) \\
&= \ln(\theta) \times \sum_{i=1}^n I_{0 \leq x_i < 1}(x_i) + \ln(1- \theta) \times (n - \sum_{i=1}^n I_{0 \leq x_i < 1}(x_i))
\end{align}
$$
令：
$$\frac{\sum_{i=1}^n I_{0 \leq x_i < 1}(x_i)}{\theta} - \frac{n -\sum_{i=1}^n I_{0 \leq x_i < 1}(x_i)}{1-\theta} = 0$$
$$(1-\theta) \times \sum_{i=1}^n I_{0 \leq x_i < 1}(x_i) = \theta \times(n -\sum_{i=1}^n I_{0 \leq x_i < 1}(x_i))$$

$$\theta = \frac{1}{n}\sum_{i=1}^n I_{0 \leq x_i < 1}(x_i)$$
# 14

$$\begin{cases}
\widehat{\mu}_{1}=\overline{x} \\
\widehat{\mu}_{2}=\overline{y} \\
\widehat{\sigma}^{2}=\frac{1}{n_{1}+n_{2}}\left[\left(n_{1}-1\right)S_{x}^{2}+\left(n_{2}-1\right)S_{y}^{2}\right]
\end{cases}$$

# 19
## part 1
$$Var(S^2) = \frac{2\sigma^4}{n-1}$$
$$b(S^2, \sigma^2) = 0$$
$$MSE(S^2) = \frac{2\sigma^4}{n-1}$$
$$Var(\frac{1}{\sigma^{2}}\sum_{i=1}^{n}\left(X_{i}-\mu\right)^{2}) = 2n$$
## part 2
$$Var(\hat\sigma_2^2) = \frac{2\sigma^4}{n}$$

$$b(\hat\sigma_2^2, \sigma^2) = 0$$

$$MSE(\hat\sigma_2^2) = \frac{2\sigma^4}{n}$$

## part 3

$$Var(\hat\sigma_3^2) = Var(\frac{n-1}{n}S^2) = \frac{2(n-1)\sigma^4}{n^2}$$

$$b(\hat\sigma_3^2, \sigma^2) = E(\hat\sigma_3^2) - \sigma^2 = \frac{n-1}{n}\sigma^2 - \sigma^2 = -\frac{\sigma^2}{n}$$

$$MSE(\hat\sigma_3^2) = \frac{2(n-1)\sigma^4}{n^2} + \frac{\sigma^4}{n^2} = \frac{(2n - 1)\sigma^4}{n^2}$$

## ans

$\hat\sigma_3^2$最好，$\hat\sigma_2^2$次之，$S^2$最差
# 25


# 32
# 34


# 45


# 48

















