

# 1

势函数:
$$g(p) = 1 - (1 - p)^3$$

第一类错误:
$$\alpha(\frac 1 2) = 1 - (\frac 1 2 ) ^ 3 = \frac 7 8$$
第二类错误:
$$\beta(\frac 3 4) = (\frac 1 4 ) ^ 3 = \frac 1 {64}$$
势:
$$\gamma(\frac 3 4) = \frac {63} {64}$$


# 2

$$x = \sum_{i=1}^n x_i \sim P(n\lambda)$$
$$P(x = k) = \frac{(n\lambda)^k}{k!}e^{-n\lambda},k=0,1,\cdots$$


势函数:
$$g(\lambda) = 1 - P(x=0) P(x=1) P(x=2) = 1 - (1 + n\lambda + \frac{n^2\lambda^2} 2)e^{-n\lambda}$$

第一类错误:
$$\alpha(\frac 1 2) = 1 - (1 + \frac n 2 + \frac{n^2} 8)e^{-\frac n 2}$$
第二类错误:
$$\beta(2) = (1 + 2n + 2n^2)e^{-2n}$$

势:
$$\gamma(2) = 1 - (1 + 2n + 2n^2)e^{-2n}$$



# 15

设拒绝域:
$$W = \{ (x_1, x_2, \cdots, x_n): \overline x \geq c \}$$

设:
$$z=\frac{\overline{x}-\mu_{0}}{\sigma_0/\sqrt{n}}$$

当$H_0$成立时,有:
$$z \sim N(0,1)$$

$$\alpha(\mu_0) = P_{\mu_0}(\frac{\overline{x}-\mu_{0}}{\sigma_0/\sqrt{n}} \geq 
\frac{c-\mu_{0}}{\sigma_0/\sqrt{n}}) = \alpha$$
$$\frac{c-\mu_{0}}{\sigma/\sqrt{n}} = z_{1- \alpha}$$

因此拒绝域为:
$$W = \{ (x_1, x_2, \cdots, x_n): \frac{\overline{x}-\mu_{0}}{\sigma_0/\sqrt{n}} \geq z_{1- \alpha} \}$$

$$\begin{align}
\beta(\mu) 
& = 1 - P_\mu\left(\frac{\overline{x}-\mu_{0}}{\sigma_0/\sqrt{n}} \geq z_{1- \alpha}\right) \\
& = 1 - P_\mu\left(\frac{\overline{x}-\mu}{\sigma_0/\sqrt{n}} \geq z_{1- \alpha} - \frac{\mu-\mu_0}{\sigma_0/\sqrt{n}} \right) \\
& = \Phi \left(z_{1- \alpha} - \frac{\mu-\mu_0}{\sigma_0/\sqrt{n}} \right), \mu \geq \mu_0 + a_0\sigma_0
\end{align}$$

令
$$\beta(\mu) = \Phi \left(z_{1- \alpha} - \frac{\mu-\mu_0}{\sigma_0/\sqrt{n}} \right) \leq \beta$$

有
$$z_{1- \alpha} - \frac{\mu-\mu_0}{\sigma_0/\sqrt{n}} \leq z_\beta$$
$$n \geq \left( \frac {\sigma_0(z_{1-\alpha} - z_\beta)} {\mu - \mu_0} \right) ^2 
\geq \frac {(z_{1-\alpha} - z_\beta)^2} {a_0^2}$$

于是得到
$$n_{min} = \left\lfloor \frac {(z_{1-\alpha} - z_\beta)^2} {a_0^2} \right\rfloor$$


# 29

$$f(x)=\frac{1}{\sqrt{2\pi}\sigma}\exp\left\{-\frac{(x-\mu)^2}{2\sigma^2}\right\}$$


$$L(x, \theta) = \frac{1}{(\sqrt{2\pi}\sigma)^n} 
\exp\left\{-\sum_{i=1}^n \frac{(x_i-\mu)^2}{2\sigma^2}\right\}$$
$$\sup_{\theta\in\Theta}\left\{p\left(x_{1},\cdots,x_{n};\theta\right)\right\}
= \frac{1}{\left(\sqrt{2\pi} \hat\sigma \right)^n}
\exp\left\{ -\frac n 2 \right\}, \hat\sigma^2 = \frac 1 n \sum_{i=1}^n (x_i - \overline x)^2$$

$$\sup_{\theta\in\Theta_{0}}\left\{p\left(x_{1},\cdots,x_{n};\theta\right)\right\}
= \frac{1}{\left(\sqrt{2\pi} \hat\sigma_0 \right)^n}
\exp\left\{ -\frac n 2 \right\}, $$
$$\hat\sigma_0^2 = \frac 1 n \sum_{i=1}^n (x_i - \min(\mu_0, \overline x))^2$$

$$\lambda(x) = \left(\frac {\hat\sigma_0^2} {\hat\sigma^2} \right) ^ {\frac n 2} 
= \frac {\sum_{i=1}^n (x_i - \min(\mu_0, \overline x))^2} {\sum_{i=1}^n (x_i - \overline x)^2}$$

$$P(\overline x > \mu_0) =  $$

$$P(\lambda(x) > c) = $$

TODO

# 33 






# 36

# 40























